code/experimental/poly1305/Hacl.Impl.Poly1305.fsti
@@ -51,7 +51,8 @@ val poly1305_update:
     (ensures  fun h0 _ h1 ->
       modifies (loc ctx) h0 h1 /\
       state_inv_t #s h1 ctx /\
-      as_get_acc h1 ctx == S.poly #(width s) (as_seq h0 text) (as_get_acc h0 ctx) (as_get_r h0 ctx))
+      Lib.Sequence.index (as_get_acc h1 ctx) 0 ==
+      S.poly_update #(width s) (as_seq h0 text) (as_get_acc h0 ctx) (as_get_r h0 ctx))
 
 inline_for_extraction
 val poly1305_finish:
@@ -66,7 +67,7 @@ val poly1305_finish:
       state_inv_t #s h ctx)
     (ensures  fun h0 _ h1 ->
       modifies (loc tag |+| loc ctx) h0 h1 /\
-      as_seq h1 tag == S.finish #(width s) (as_seq h0 key) (as_get_acc h0 ctx))
+      as_seq h1 tag == S.finish (as_seq h0 key) (Lib.Sequence.index (as_get_acc h0 ctx) 0))
 
 inline_for_extraction
 val poly1305_mac:
