code/experimental/poly1305/Hacl.Poly1305_32.fst
@@ -14,6 +14,9 @@ let blocklen = 16ul
 
 type poly1305_ctx = lbuffer (Lib.IntVector.vec_t U64 1) 25ul
 
+unfold
+let op_String_Access #a #len = Lib.Sequence.index #a #len
+
 val poly1305_init:
     ctx:poly1305_ctx
   -> key:lbuffer uint8 32ul
@@ -38,7 +41,8 @@ val poly1305_update_blocks:
     (ensures  fun h0 _ h1 ->
       modifies (loc ctx) h0 h1 /\
       state_inv_t #M32 h1 ctx /\
-      as_get_acc h1 ctx == S.poly (as_seq h0 text) (as_get_acc h0 ctx) (as_get_r h0 ctx))
+      (as_get_acc h1 ctx).[0] ==
+      S.poly_update (as_seq h0 text) (as_get_acc h0 ctx) (as_get_r h0 ctx))
 let poly1305_update_blocks ctx len text =
   poly1305_update #M32 ctx len text
 
@@ -53,7 +57,8 @@ val poly1305_update_padded:
     (ensures  fun h0 _ h1 ->
       modifies (loc ctx) h0 h1 /\
       state_inv_t #M32 h1 ctx /\
-      as_get_acc h1 ctx == S.poly (as_seq h0 text) (as_get_acc h0 ctx) (as_get_r h0 ctx))
+      (as_get_acc h1 ctx).[0] ==
+      S.poly_update (as_seq h0 text) (as_get_acc h0 ctx) (as_get_r h0 ctx))
 let poly1305_update_padded ctx len text =
   poly1305_update #M32 ctx len text
 
@@ -68,7 +73,8 @@ val poly1305_update_last:
     (ensures  fun h0 _ h1 ->
       modifies (loc ctx) h0 h1 /\
       state_inv_t #M32 h1 ctx /\
-      as_get_acc h1 ctx == S.poly (as_seq h0 text) (as_get_acc h0 ctx) (as_get_r h0 ctx))
+      (as_get_acc h1 ctx).[0] ==
+      S.poly_update (as_seq h0 text) (as_get_acc h0 ctx) (as_get_r h0 ctx))
 let poly1305_update_last ctx len text =
   poly1305_update #M32 ctx len text
 
@@ -83,7 +89,7 @@ val poly1305_finish:
       state_inv_t h ctx)
     (ensures  fun h0 _ h1 ->
       modifies (loc tag |+| loc ctx) h0 h1 /\
-      as_seq h1 tag == S.finish (as_seq h0 key) (as_get_acc h0 ctx))
+      as_seq h1 tag == S.finish (as_seq h0 key) (as_get_acc h0 ctx).[0])
 let poly1305_finish tag k ctx =
   poly1305_finish #M32 tag k ctx
 
